imports.v
@@ -1,0 +1,7 @@
+From Coq Require Export ssreflect ssrbool.
+From Coq Require Export Logic.PropExtensionality
+  (propositional_extensionality) Program.Basics (const).
+From Equations Require Export Equations.
+From Hammer Require Export Tactics.
+From stdpp Require Export relations (rtc, rtc_transitive, rtc_once, rtc_inv, rtc(..), diamond, confluent, diamond_confluent).
+Require Export Psatz.
